theories/Problems/cbvLambda.v
@@ -4,4 +4,6 @@ From Undecidability.L Require Import L.
 
 (* Call-by-Value Lambda Calculus as a Model of Computation in Coq. Yannick Forster and Gert Smolka. Journal of Automated Reasoning (2018). https://www.ps.uni-saarland.de/extras/L-computability/ *)
 
-About eva. (* Halting problem for call-by-value lambda-calculus *)
+Definition HaltL s := exists t, eval s t. (* Halting problem for call-by-value lambda-calculus *)
+
+Definition HaltLclosed (s : {s : term | closed s}) := exists t, eval (proj1_sig s) t. (* Halting problem for call-by-value lambda-calculus *)
